Korrespondenzprinzip \cite[Glg. 2.13]{qm}
\begin{itemize}
    \item Observablen sind hermitsche Operatoren
\end{itemize}
Dualraum \cite[Glg. A.32]{qm}
\begin{equation*}
	\hat{A}\ket{v}=\ket{w} \qquad \Leftrightarrow \qquad \bra{v}\hat{A}^\dagger=\bra{w}
\end{equation*}
Matrixdarstellung \cite[S. A.16]{qm}
\begin{equation*}
	\hat{O} = \sum_{ij}O_{ij}^{(e)}\ketbra{e_i}{e_j} \qquad \Leftrightarrow \qquad O_{ij}^{(e)}=\braket{e_i|\hat{O}|e_j}
\end{equation*}
Spur \cite[Def. A.19, Thm. A.4]{qm}
\begin{equation*}
	\tr\hat{O} = \sum_i\braket{e_i|\hat{O}|e_i} \qquad \text{(basisunabh√§ngig)}
\end{equation*}
Kommutator, Antikommutator \cite[Glg. A.22, S. 51]{qm}
\begin{equation*}
	[\hat{A},\hat{B}]=\hat{A}\hat{B}-\hat{B}\hat{A} \qquad \{\hat{A},\hat{B}\}=\hat{A}\hat{B}+\hat{B}\hat{A}
\end{equation*}
Produktregel \cite[Glg. A.23]{qm}
\begin{equation*}
	[\hat{A}\hat{B},\hat{C}] = \hat{A}[\hat{B},\hat{C}] + [\hat{A},\hat{C}]\hat{B}
\end{equation*}
Unbestimmtheitsrelation \cite[Glg. A.160]{qm}
\begin{equation*}
	\braket{(\Delta\hat{A})^2}\braket{(\Delta\hat{B})^2} \geq \frac{|\braket{[\hat{A},\hat{B}]}|^2}{4}
\end{equation*}
